fpiwrgnprgnwpr

.lake/build/ir/Games/gameLib_fixfix/Basic.c
@@ -13,6 +13,7 @@
 #ifdef __cplusplus
 extern "C" {
 #endif
+LEAN_EXPORT lean_object* l___private_Games_gameLib__fixfix_Basic_0__History__on__turn_match__1_splitter(lean_object*);
 LEAN_EXPORT lean_object* l_Symm__Game__World_history__on__turn(lean_object*, lean_object*);
 LEAN_EXPORT lean_object* l_State__from__history___rarg(lean_object*, lean_object*, lean_object*, lean_object*);
 LEAN_EXPORT lean_object* l_Symm__Game_history__on__turn___rarg___boxed(lean_object*, lean_object*);
@@ -33,6 +34,8 @@ LEAN_EXPORT lean_object* l_Symm__Game__World_toGame__World___elambda__1(lean_obj
 LEAN_EXPORT lean_object* l_Symm__Game_toGame___rarg(lean_object*);
 LEAN_EXPORT uint8_t l_instDecidablePredNatTurn__fst(lean_object*);
 uint8_t l_instDecidableNot___rarg(uint8_t);
+LEAN_EXPORT lean_object* l___private_Games_gameLib__fixfix_Basic_0__History__on__turn_match__1_splitter___rarg___boxed(lean_object*, lean_object*, lean_object*);
+LEAN_EXPORT lean_object* l___private_Games_gameLib__fixfix_Basic_0__History__on__turn_match__1_splitter___rarg(lean_object*, lean_object*, lean_object*);
 LEAN_EXPORT lean_object* l_Game_state__on__turn___rarg___boxed(lean_object*, lean_object*);
 LEAN_EXPORT lean_object* l_History__on__turn(lean_object*, lean_object*);
 LEAN_EXPORT lean_object* l_Game__World_history__on__turn___rarg___boxed(lean_object*, lean_object*, lean_object*, lean_object*);
@@ -732,6 +735,46 @@ _start:
 lean_object* x_3; 
 x_3 = lean_alloc_closure((void*)(l_State__from__history___rarg), 4, 0);
 return x_3;
+}
+}
+LEAN_EXPORT lean_object* l___private_Games_gameLib__fixfix_Basic_0__History__on__turn_match__1_splitter___rarg(lean_object* x_1, lean_object* x_2, lean_object* x_3) {
+_start:
+{
+lean_object* x_4; uint8_t x_5; 
+x_4 = lean_unsigned_to_nat(0u);
+x_5 = lean_nat_dec_eq(x_1, x_4);
+if (x_5 == 0)
+{
+lean_object* x_6; lean_object* x_7; lean_object* x_8; 
+x_6 = lean_unsigned_to_nat(1u);
+x_7 = lean_nat_sub(x_1, x_6);
+x_8 = lean_apply_1(x_3, x_7);
+return x_8;
+}
+else
+{
+lean_dec(x_3);
+lean_inc(x_2);
+return x_2;
+}
+}
+}
+LEAN_EXPORT lean_object* l___private_Games_gameLib__fixfix_Basic_0__History__on__turn_match__1_splitter(lean_object* x_1) {
+_start:
+{
+lean_object* x_2; 
+x_2 = lean_alloc_closure((void*)(l___private_Games_gameLib__fixfix_Basic_0__History__on__turn_match__1_splitter___rarg___boxed), 3, 0);
+return x_2;
+}
+}
+LEAN_EXPORT lean_object* l___private_Games_gameLib__fixfix_Basic_0__History__on__turn_match__1_splitter___rarg___boxed(lean_object* x_1, lean_object* x_2, lean_object* x_3) {
+_start:
+{
+lean_object* x_4; 
+x_4 = l___private_Games_gameLib__fixfix_Basic_0__History__on__turn_match__1_splitter___rarg(x_1, x_2, x_3);
+lean_dec(x_2);
+lean_dec(x_1);
+return x_4;
 }
 }
 lean_object* initialize_Init(uint8_t builtin, lean_object*);
